src/Lib/VstCallback.v
@@ -1,0 +1,41 @@
+Require Import Core.Core.
+Require Import VST.floyd.proofauto.
+Require Import Clight.asn_application.
+
+Definition Vprog : varspecs. mk_varspecs prog. Defined.
+Instance CompSpecs : compspecs. make_compspecs prog. Defined.
+
+Open Scope Z.
+
+Section Encoder_callback.
+
+Definition enc_key := Tstruct _overrun_encoder_key noattr.
+
+Definition constr_enc_key buf size comp_size : reptype enc_key := 
+  (buf, (Vint (Int.repr size), Vint (Int.repr comp_size))).
+
+Definition callback : funspec :=
+    WITH data : list byte, data_p : val, size : Z, key_p : val
+    PRE[tptr tvoid, tuint, tptr tvoid]
+      PROP()
+      PARAMS(data_p; Vint (Int.repr size); key_p)
+      GLOBALS()
+      SEP((*data_at Tsh (tarray tint size) _ data_p;
+          data_at Tsh enc_key (constr_enc_key) key_p; *))
+    POST[tint]
+      PROP()
+      LOCAL(temp __res (Vint (Int.repr 0)))
+      SEP().
+
+Definition callback_spec : ident * funspec :=
+  DECLARE _overrun_encoder_cb callback.
+
+Definition Gprog := ltac:(with_library prog [callback_spec]).
+
+Theorem bool_der_encode : semax_body Vprog Gprog f_overrun_encoder_cb 
+                                     callback_spec.
+Proof.
+  start_function.
+Admitted.
+
+End Encoder_callback.
